\documentclass[a4paper]{article}

\usepackage[T1]{fontenc}	
\usepackage{amsmath}

\begin{document}
 
\section*{Random Number Generation}

\subsection*{1)}

\subsubsection*{a)}

\begin{equation}
     \begin{gathered}
        F_{X|x\in{I}}(x) = P(X < x | X \in I) \\
        = P(F_X^{-1}(U) < x | F_X^{-1}(U) \in I) \\
        = P(F_X^{-1}((F_X(b)-F_X(a))U+F_X(a)) < x) \\
        = P((F_X(b)-F_X(a))U + F_X(a) < F_X(x)) \\
        = P(U < \frac{F_X(x)-F_X(a)}{F_X(b)-F_X(a)})
        = \frac{F_X(x)-F_X(a)}{F_X(b)-F_X(a)}
     \end{gathered}
\end{equation}

Annat sätt att räkna

\begin{equation}
    F_{X|\in{I}}(x) = \frac{\int_a^xf_X(x)dx}{c} = \frac{\int_a^xf_X(x)dx}{\int_a^bf_X(x)dx} = \frac{F_X(x)-F_X(a)}{F_X(b)-F_X(a)}
\end{equation}

\begin{equation}
    f_{X|\in{I}}(x) = \frac{dF_{X|\in{I}}(x)}{dx} = \frac{f_X(x)}{F_X(b)-F_X(a)}
\end{equation}

\subsubsection*{b)}

\begin{equation}
    F_{X|\in{I}}^{-1}(x) = F_X^{-1}((F_X(b)- F_X(a))x + F_X(a))
\end{equation}


\end{document}
